Start working thought semantic relation properties

compiler1/semantics/closRelationScript.sml
@@ -2,6 +2,10 @@ open preamble closLangTheory closSemTheory closPropsTheory;
 
 val _ = new_theory "closRelation";
 
+val clock_lemmas = Q.prove (
+`!s. (s with clock := s.clock) = s`,
+ rw [state_component_equality]);
+
 val is_closure_def = Define `
 (is_closure (Closure _ _ _ _ _) ⇔ T) ∧
 (is_closure (Recclosure _ _ _ _ _) ⇔ T) ∧
@@ -78,7 +82,7 @@ val val_rel_def = tDefine "val_rel" `
                  state_rel i' s s' ∧
                  LIST_REL (val_rel i') env env'
                  ⇒
-                 exec_rel i ([e],env,s) ([e'],env',s')
+                 exec_rel i' ([e],env,s) ([e'],env',s')
                else
                  T)
            s.code s'.code ∧
@@ -100,7 +104,259 @@ val val_rel_def = tDefine "val_rel" `
  >- (Induct_on `vs` >>
      rw [v_size_def] >>
      res_tac >>
-     decide_tac) >>
-     cheat); 
+     decide_tac));
+
+val res_rel_def = Define `
+(res_rel (Rval vs, s) (Rval vs', s') ⇔
+  s.clock = s'.clock ∧
+  state_rel s.clock s s' ∧ 
+  LIST_REL (val_rel s.clock) vs vs') ∧ 
+(res_rel (Rerr (Rraise v), s) (Rerr (Rraise v'), s') ⇔
+  s.clock = s'.clock ∧
+  state_rel s.clock s s' ∧ 
+  val_rel s.clock v v') ∧ 
+(res_rel (Rerr (Rabort Rtimeout_error), s) (Rerr (Rabort Rtimeout_error), s') ⇔
+  state_rel s.clock s s') ∧
+(res_rel (Rerr (Rabort Rtype_error), _) _ ⇔ T) ∧
+(res_rel _ _ ⇔ F)`;
+
+val res_rel_rw = Q.store_thm ("res_rel_rw",
+`(res_rel (Rval vs, s) x ⇔ 
+  ?vs' s'. x = (Rval vs', s') ∧
+  LIST_REL (val_rel s.clock) vs vs' ∧ 
+  state_rel s.clock s s' ∧
+  s.clock = s'.clock) ∧
+ (res_rel (Rerr (Rraise v), s) x ⇔ 
+  ?v' s'. x = (Rerr (Rraise v'), s') ∧ 
+  val_rel s.clock v v' ∧ 
+  state_rel s.clock s s' ∧ 
+  s.clock = s'.clock) ∧
+ (res_rel (Rerr (Rabort Rtimeout_error), s) x ⇔ 
+   ?s'. x = (Rerr (Rabort Rtimeout_error), s') ∧ state_rel s.clock s s') ∧
+ (res_rel (Rerr (Rabort Rtype_error), s) x ⇔ T)`,
+ rw [] >>
+ Cases_on `x` >>
+ Cases_on `q` >>
+ TRY (Cases_on `e`) >>
+ TRY (Cases_on `a`) >>
+ fs [res_rel_def] >>
+ metis_tac []);
+
+val exp_rel_def = Define `
+exp_rel es es' ⇔
+  !i env env' s s'.
+    state_rel i s s' ∧
+    LIST_REL (val_rel i) env env' ⇒
+    exec_rel i (es, env, s) (es', env', s')`;
+
+val val_rel_ind = theorem "val_rel_ind";
+
+val fun_lemma = Q.prove (
+`!f x. (\a a'. f x a a') = f x`,
+ rw [FUN_EQ_THM]);
+
+fun find_clause good_const = 
+  good_const o fst o strip_comb o fst o dest_eq o snd o strip_forall o concl;
+
+val result_store_cases = Q.store_thm ("result_store_cases",
+`!r. ?s. 
+  (?vs. r = (Rval vs, s)) ∨
+  (?v. r = (Rerr (Rraise v), s)) ∨
+  (r = (Rerr (Rabort Rtimeout_error), s)) ∨
+  (r = (Rerr (Rabort Rtype_error), s))`,
+ Cases_on `r` >>
+ rw [] >>
+ qexists_tac `r'` >>
+ rw [] >>
+ Cases_on `q` >>
+ rw [] >>
+ Cases_on `e` >>
+ rw [] >>
+ Cases_on `a` >>
+ rw []);
+
+val val_rel_rw = 
+  let val clauses = CONJUNCTS val_rel_def
+      fun good_const x = same_const ``val_rel`` x
+  in
+    SIMP_RULE (srw_ss()) [fun_lemma, AND_IMP_INTRO, is_closure_def]
+        (LIST_CONJ (List.filter (find_clause good_const) clauses))
+  end;
+
+val _ = save_thm ("val_rel_rw", val_rel_rw);
+
+val state_rel_rw = 
+  let val clauses = CONJUNCTS val_rel_def
+      fun good_const x = same_const ``state_rel`` x orelse same_const ``ref_v_rel`` x
+  in
+    SIMP_RULE (srw_ss()) [fun_lemma] 
+         (LIST_CONJ (List.filter (find_clause good_const) clauses))
+  end;
+
+val _ = save_thm ("state_rel_rw", state_rel_rw);
+
+val exec_rel_rw = Q.store_thm ("exec_rel_rw",
+`(exec_rel i (es,env,s) (es',env',s') ⇔
+  !i'. i' ≤ i ⇒
+    res_rel (evaluate (es,env,s with clock := i')) 
+            (evaluate (es',env',s' with clock := i'))) ∧
+ (exec_cl_rel i (cl,args,s) (cl',args',s') ⇔
+  !i'. i' ≤ i ⇒
+    res_rel (evaluate_app NONE cl args (s with clock := i')) 
+            (evaluate_app NONE cl' args' (s' with clock := i')))`,
+ rw [] >>
+ ONCE_REWRITE_TAC [val_rel_def] >>
+ rw [fun_lemma] >>
+ eq_tac >>
+ fs [] >>
+ rw []
+ >- (strip_assume_tac (Q.ISPEC `evaluate (es,env,s with clock := i')`
+                         result_store_cases) >>
+     strip_assume_tac (Q.ISPEC `evaluate (es',env',s' with clock := i')` 
+                         result_store_cases) >>
+     simp [res_rel_rw] >>
+     res_tac >>
+     fs [] >>
+     rfs [])
+ >- (first_x_assum (qspec_then `i'` mp_tac) >>
+     rw [] >>
+     strip_assume_tac (Q.ISPEC `evaluate (es,env,s with clock := i')` 
+                         result_store_cases) >>
+     strip_assume_tac (Q.ISPEC `evaluate (es',env',s' with clock := i')` 
+                         result_store_cases) >>
+     fs [] >>
+     rw [] >>
+     fs [res_rel_rw] >>
+     fs [])
+ >- (strip_assume_tac (Q.ISPEC `evaluate_app NONE cl args (s with clock := i')`
+                         result_store_cases) >>
+     strip_assume_tac (Q.ISPEC `evaluate_app NONE cl' args' (s' with clock := i')` 
+                         result_store_cases) >>
+     simp [res_rel_rw] >>
+     res_tac >>
+     fs [] >>
+     rfs [])
+ >- (first_x_assum (qspec_then `i'` mp_tac) >>
+     rw [] >>
+     strip_assume_tac (Q.ISPEC `evaluate_app NONE cl args (s with clock := i')` 
+                         result_store_cases) >>
+     strip_assume_tac (Q.ISPEC `evaluate_app NONE cl' args' (s' with clock := i')` 
+                         result_store_cases) >>
+     fs [] >>
+     rw [] >>
+     fs [res_rel_rw] >>
+     fs []));
+
+val val_rel_mono = Q.store_thm ("val_rel_mono",
+`(!i v v'. val_rel i v v' ⇒ ∀i'. i' ≤ i ⇒ val_rel i' v v') ∧
+ (!i st st'. exec_rel i st st' ⇒ !i'. i' ≤ i ⇒ exec_rel i' st st') ∧
+ (!i st st'. exec_cl_rel i st st' ⇒ !i'. i' ≤ i ⇒ exec_cl_rel i' st st') ∧
+ (!i rv rv'. ref_v_rel i rv rv' ⇒ !i'. i' ≤ i ⇒ ref_v_rel i' rv rv') ∧
+ (!i s s'. state_rel i s s' ⇒ !i'. i' ≤ i ⇒ state_rel i' s s')`,
+ ho_match_mp_tac val_rel_ind >>
+ rw [val_rel_rw, exec_rel_rw] >>
+ fs [is_closure_def] >>
+ rw []
+ >- (fs [LIST_REL_EL_EQN] >>
+     rw [] >>
+     metis_tac [MEM_EL])
+ >- (`i''' < i ∧ i'' < i` by decide_tac >>
+     metis_tac [])
+ >- (`i''' < i ∧ i'' < i` by decide_tac >>
+     metis_tac [])
+ >- (`i'' ≤ i` by decide_tac >>
+     metis_tac [])
+ >- (`i'' ≤ i` by decide_tac >>
+     metis_tac [])
+ >- fs [state_rel_rw]
+ >- (fs [state_rel_rw, LIST_REL_EL_EQN] >>
+     rw [] >>
+     metis_tac [MEM_EL])
+ >- fs [state_rel_rw]
+ >- fs [state_rel_rw]
+ >- (qpat_assum `state_rel P1 P2 P3` mp_tac >>
+     ONCE_REWRITE_TAC [state_rel_rw] >>
+     rw []
+     >- (fs [LIST_REL_EL_EQN] >>
+         rw [] >>
+         metis_tac [MEM_EL, OPTREL_MONO])
+     >- metis_tac [fmap_rel_mono]
+     >- (imp_res_tac ((GEN_ALL o SIMP_RULE (srw_ss()) [AND_IMP_INTRO]) fmap_rel_mono) >>
+         pop_assum kall_tac >>
+         pop_assum match_mp_tac >> 
+         rw [] >>
+         PairCases_on `x` >>
+         PairCases_on `y` >>
+         fs [] >>
+         rw [] >>
+         `i'' < i` by decide_tac >>
+         metis_tac [])));
+  
+val val_rel_mono_list = Q.store_thm ("val_rel_mono_list",
+`!i i' vs1 vs2.
+  i' ≤ i ∧ LIST_REL (val_rel i) vs1 vs2
+  ⇒
+  LIST_REL (val_rel i') vs1 vs2`,
+ rw [LIST_REL_EL_EQN] >>
+ metis_tac [val_rel_mono]);
+
+val state_rel_clock = Q.store_thm ("state_rel_clock[simp]",
+`!c1 c2 s s'.
+  (state_rel c1 (s with clock := c2) s' ⇔ state_rel c1 s s') ∧
+  (state_rel c1 s (s' with clock := c2) ⇔ state_rel c1 s s')`,
+ rw [] >>
+ ONCE_REWRITE_TAC [state_rel_rw] >>
+ rw []);
+
+val compat_nil = Q.store_thm ("compat_nil",
+`exp_rel [] []`,
+ rw [exp_rel_def, exec_rel_rw, evaluate_def, res_rel_rw] >>
+ metis_tac [val_rel_mono]);
+
+(* compat_cons, or compat_append? *)
+
+val compat_var = Q.store_thm ("compat_var",
+`!n. exp_rel [Var n] [Var n]`,
+ rw [exp_rel_def, exec_rel_rw, evaluate_def] >>
+ rw [res_rel_rw] >>
+ fs [LIST_REL_EL_EQN] >>
+ metis_tac [MEM_EL, val_rel_mono]);
+
+val compat_if = Q.store_thm ("compat_if",
+`!e1 e2 e3 e1' e2' e3'.
+  exp_rel [e1] [e1'] ∧
+  exp_rel [e2] [e2'] ∧
+  exp_rel [e3] [e3']
+  ⇒
+  exp_rel [If e1 e2 e3] [If e1' e2' e3']`,
+ rw [Boolv_def, exp_rel_def, exec_rel_rw, evaluate_def] >>
+ fs [PULL_FORALL] >>
+ imp_res_tac val_rel_mono >>
+ imp_res_tac val_rel_mono_list >>
+ last_x_assum (qspecl_then [`i'`, `env`, `env'`, `s`, `s'`, `i'`] mp_tac) >>
+ reverse (strip_assume_tac (Q.ISPEC `evaluate ([e1],env,s with clock := i')`
+                         result_store_cases)) >>
+ rw [res_rel_rw] >>
+ simp []
+ >- metis_tac [] >>
+ `?v v'. vs = [v] ∧ vs' = [v']` by metis_tac [evaluate_SING] >>
+ fs [] >>
+ rw [] >>
+ fs [val_rel_rw]
+ >- (imp_res_tac evaluate_clock >>
+     fs [] >>
+     metis_tac [val_rel_mono_list, LESS_EQ_REFL, clock_lemmas])
+ >- (Cases_on `v'` >>
+     fs [val_rel_rw] >>
+     fs [])
+ >- (imp_res_tac evaluate_clock >>
+     fs [] >>
+     metis_tac [val_rel_mono_list, LESS_EQ_REFL, clock_lemmas])
+ >- (Cases_on `v'` >>
+     fs [val_rel_rw] >>
+     fs []));
+
+
+
 
 val _ = export_theory ();
